i2c/i2cCircuitCompileScript.sml
@@ -5,56 +5,6 @@ open i2cCircuitTheory;
 
 val _ = new_theory "i2cCircuitCompile";
 
-    (*
-Theorem i2c_circuit_alt_def:
-i2c_circuit =
-     mk_module
-       (procs
-        ([i2c_core_counter_ff; i2c_core_stretch_idle_cnt_ff;
-          fmt_fifo_rptr_ff; fmt_fifo_regfile_ff; i2c_core_rx_fifo_wptr_ff;
-          fmt_fifo_wptr_ff; bit_index_ff; pend_restart_ff; byte_index_ff;
-          i2c_core_rx_fifo_rptr_ff; i2c_core_rx_fifo_regfile; i2c_core_ff;
-          i2c_reg_top_ff]))
-       (procs
-        ([i2c_reg_top_comb_1;
-          i2c_core_rx_fifo_counter_wptr_wrap_comb;
-            i2c_core_rx_fifo_counter_wptr_wrap_cnt_comb; i2c_core_delay_comb;
-            i2c_core_curr_delay_comb; i2c_core_load_tcount_comb;
-            i2c_core_stretch_en_comb; i2c_core_scl_d_comb;
-            i2c_core_next_stretch_idle_cnt; i2c_core_next_counter;
-            i2c_core_next_state; fmt_fifo_reset; counter_gt_one_comb;
-            fmt_fifo_rdata; fmt_fifo_rready; fmt_fifo_empty;
-            fmt_fifo_counter_rptr_wrap; fmt_fifo_counter_rptr_wrap_cnt;
-            fmt_fifo_wvalid; fmt_fifo_full; fmt_fifo_incr_wptr;
-            fmt_fifo_wdata; fmt_fifo_counter_wptr_wrap;
-            fmt_fifo_counter_wptr_wrap_cnt; i2c_core_log_start_comb;
-            i2c_core_log_stop_comb; fmt_fifo_rvalid;
-            fmt_fifo_flag_start_before; fmt_fifo_flag_stop_after;
-            fmt_fifo_flag_read_bytes; fmt_byte; req_restart; bit_clr;
-            bit_decr; i2c_core_next_scl_rx_val_comb; i2c_core_byte_clr_comb;
-            i2c_core_byte_num_comb; i2c_core_next_byte_index_comb;
-            fifo_depth; i2c_core_read_byte_clr_comb;
-            i2c_core_shift_data_en_comb; i2c_core_next_sda_rx_val_comb;
-            i2c_core_next_read_byte_comb; i2c_core_rx_fifo_reset_comb;
-            i2c_core_rx_fifo_rdata_comb; i2c_core_rx_fifo_rready_comb;
-            i2c_core_rx_fifo_empty_comb; i2c_core_rx_fifo_incr_rptr_comb;
-            i2c_core_rx_fifo_counter_rptr_wrap_comb;
-            i2c_core_rx_fifo_counter_rptr_wrap_cnt_comb;
-            i2c_core_rx_fifo_wvalid_comb; i2c_core_rx_fifo_wdata_comb;
-            i2c_core_rx_fifo_full_comb; i2c_core_rx_fifo_incr_wptr_comb;
-            hw2reg_intr_state_nak_de_comb; next_intr_nak_comb;
-            hw2reg_intr_state_cmd_complete_de_comb;
-            hw2reg_intr_state_cmd_complete_d_comb;
-            next_intr_cmd_complete_comb; next_pend_restart_comb;
-            next_trans_started_comb; next_bit_index_comb;
-            i2c_reg_top_comb_2]))
-       i2c_circuit_init
-Proof
-  rw [i2c_circuit_def, i2c_core_ffs1_def, i2c_core_combs_def]
-QED
-    *)
-
-
 Theorem i2c_circuit_alt_def:
 i2c_circuit =
      mk_module
@@ -63,16 +13,25 @@ i2c_circuit =
           i2c_core_tx_fifo_rptr_ff; i2c_core_tx_fifo_regfile; i2c_core_tx_fifo_wptr_ff;
           i2c_core_acq_fifo_rptr_ff; i2c_core_acq_fifo_regfile; i2c_core_acq_fifo_wptr_ff;
           i2c_core_rx_fifo_rptr_ff; i2c_core_rx_fifo_regfile; i2c_core_rx_fifo_wptr_ff;
-          i2c_core_sync_ff; i2c_core_ff; i2c_core_counter_ff;
-          i2c_core_stretch_idle_cnt_ff; bit_index_ff; i2c_core_bit_idx_ff;
-          pend_restart_ff; trans_started_ff; byte_index_ff; read_byte_ff;
-          i2c_core_input_byte_ff; scl_rx_val_ff; sda_rx_val_ff; scl_i_q_ff; sda_i_q_ff;
-          i2c_core_under_rst_ff; i2c_core_rw_bit_ff; i2c_core_host_ack_ff; i2c_reg_top_ff]))
+          i2c_core_fmt_threshold_q_ff; i2c_core_rx_threshold_q_ff;
+          i2c_core_sda_rise_cnt_ff; i2c_core_intr_fmt_threshold_o_ff;
+          i2c_core_intr_rx_threshold_o_ff; i2c_core_intr_fmt_overflow_o_ff;
+          i2c_core_intr_rx_overflow_o_ff; i2c_core_intr_nak_o_ff;
+          i2c_core_intr_scl_interference_o_ff; i2c_core_intr_sda_interference_o_ff;
+          i2c_core_intr_stretch_timeout_o_ff; i2c_core_intr_sda_unstable_o_ff;
+          i2c_core_intr_cmd_complete_o_ff; i2c_core_test_tx_stretch_ff;
+          i2c_core_intr_tx_stretch_o_ff; i2c_core_intr_tx_overflow_o_ff;
+          i2c_core_test_acq_full_ff; i2c_core_intr_acq_full_o_ff;
+          i2c_core_intr_unexp_stop_o_ff; i2c_core_intr_host_timeout_o_ff;
+          i2c_core_sync_ff; i2c_core_scl_q_ff; i2c_core_sda_q_ff; i2c_core_ff;
+          i2c_core_counter_ff; i2c_core_stretch_idle_cnt_ff; bit_index_ff;
+          i2c_core_bit_idx_ff; pend_restart_ff; trans_started_ff; byte_index_ff;
+          read_byte_ff; i2c_core_input_byte_ff; scl_rx_val_ff; sda_rx_val_ff; scl_i_q_ff;
+          sda_i_q_ff; i2c_core_under_rst_ff; i2c_core_rw_bit_ff; i2c_core_host_ack_ff; i2c_reg_top_ff]))
        (procs
         ([i2c_reg_top_comb_1;
           i2c_core_target_loopback_comb; i2c_core_start_det_comb; i2c_core_stop_det_comb;
           i2c_core_address_match_comb; i2c_core_target_idle_comb; i2c_core_host_idle_comb;
-          i2c_core_event_host_timeout_comb; i2c_core_event_stretch_timeout_comb;
           fmt_fifo_reset; fmt_fifo_rdata; fmt_fifo_rready; fmt_fifo_empty;
           fmt_fifo_incr_rptr; fmt_fifo_counter_rptr_wrap; fmt_fifo_counter_rptr_wrap_cnt;
           fmt_fifo_wvalid; fmt_fifo_full; fmt_fifo_wready; fmt_fifo_incr_wptr;
@@ -80,15 +39,16 @@ i2c_circuit =
           i2c_core_delay_comb; i2c_core_curr_delay_comb; i2c_core_load_tcount_comb;
           i2c_core_log_start_comb; i2c_core_log_stop_comb; fmt_fifo_rvalid;
           fmt_fifo_flag_start_before; fmt_fifo_flag_stop_after; fmt_fifo_flag_read_bytes;
-          fmt_fifo_flag_nak_ok; i2c_core_tx_fifo_rdata_comb; i2c_core_tx_fifo_empty_comb;
-          i2c_core_tx_fifo_rvalid_comb; i2c_core_tx_fifo_full_comb;
-          i2c_core_tx_fifo_wready_comb; i2c_core_tx_fifo_depth_comb;
-          i2c_core_acq_fifo_rdata_comb; i2c_core_acq_fifo_empty_comb;
-          i2c_core_acq_fifo_rvalid_comb; i2c_core_acq_fifo_full_comb;
-          i2c_core_acq_fifo_wready_comb; i2c_core_acq_fifo_depth_comb;
-          i2c_core_tx_fifo_reset_comb; i2c_core_tx_fifo_rready_comb;
-          i2c_core_tx_fifo_wvalid_comb; i2c_core_tx_fifo_wdata_comb;
-          i2c_core_tx_fifo_incr_rptr_comb; i2c_core_tx_fifo_counter_rptr_wrap_comb;
+          fmt_fifo_flag_read_continue; fmt_fifo_flag_nak_ok; i2c_core_tx_fifo_rdata_comb;
+          i2c_core_tx_fifo_empty_comb; i2c_core_tx_fifo_rvalid_comb;
+          i2c_core_tx_fifo_full_comb; i2c_core_tx_fifo_wready_comb;
+          i2c_core_tx_fifo_depth_comb; i2c_core_acq_fifo_rdata_comb;
+          i2c_core_acq_fifo_empty_comb; i2c_core_acq_fifo_rvalid_comb;
+          i2c_core_acq_fifo_full_comb; i2c_core_acq_fifo_wready_comb;
+          i2c_core_acq_fifo_depth_comb; i2c_core_tx_fifo_reset_comb;
+          i2c_core_tx_fifo_rready_comb; i2c_core_tx_fifo_wvalid_comb;
+          i2c_core_tx_fifo_wdata_comb; i2c_core_tx_fifo_incr_rptr_comb;
+          i2c_core_tx_fifo_counter_rptr_wrap_comb;
           i2c_core_tx_fifo_counter_rptr_wrap_cnt_comb; i2c_core_tx_fifo_incr_wptr_comb;
           i2c_core_tx_fifo_counter_wptr_wrap_comb;
           i2c_core_tx_fifo_counter_wptr_wrap_cnt_comb; i2c_core_acq_fifo_reset_comb;
@@ -99,8 +59,10 @@ i2c_circuit =
           i2c_core_acq_fifo_counter_wptr_wrap_comb;
           i2c_core_acq_fifo_counter_wptr_wrap_cnt_comb; i2c_core_stretch_tx_comb;
           fmt_byte; req_restart; bit_clr; bit_decr; i2c_core_stretch_en_comb;
-          i2c_core_scl_d_comb; i2c_core_next_scl_rx_val_comb;
-          i2c_core_next_stretch_idle_cnt; i2c_core_next_counter; i2c_core_byte_clr_comb;
+          i2c_core_scl_d_comb; i2c_core_sda_d_comb; i2c_core_scl_o_comb;
+          i2c_core_sda_o_comb; i2c_core_cio_scl_o_comb; i2c_core_cio_sda_o_comb;
+          i2c_core_cio_scl_en_o_comb; i2c_core_cio_sda_en_o_comb;
+          i2c_core_next_scl_rx_val_comb; i2c_core_next_counter; i2c_core_byte_clr_comb;
           i2c_core_byte_decr_comb; i2c_core_byte_num_comb; i2c_core_next_byte_index_comb;
           fifo_depth; counter_gt_one_comb; i2c_core_next_state;
           i2c_core_read_byte_clr_comb; i2c_core_input_byte_clr_comb;
@@ -113,13 +75,56 @@ i2c_circuit =
           i2c_core_rx_fifo_wdata_comb; i2c_core_rx_fifo_full_comb;
           i2c_core_rx_fifo_wready_comb; i2c_core_rx_fifo_depth_comb;
           i2c_core_rx_fifo_incr_wptr_comb; i2c_core_rx_fifo_counter_wptr_wrap_comb;
-          i2c_core_rx_fifo_counter_wptr_wrap_cnt_comb; hw2reg_intr_state_nak_de_comb;
-          hw2reg_intr_state_nak_d_comb; next_intr_nak_comb;
-          hw2reg_intr_state_cmd_complete_de_comb; hw2reg_intr_state_cmd_complete_d_comb;
-          next_intr_cmd_complete_comb; next_pend_restart_comb; next_trans_started_comb;
-          next_bit_index_comb; i2c_core_status_fmtfull_d_comb;
-          i2c_core_status_rxfull_d_comb; i2c_core_status_fmtempty_d_comb;
-          i2c_core_status_rxempty_d_comb;
+          i2c_core_rx_fifo_counter_wptr_wrap_cnt_comb; i2c_core_fmt_threshold_d_comb;
+          i2c_core_rx_threshold_d_comb; i2c_core_en_sda_interf_det_comb;
+          i2c_core_expect_stop_comb; i2c_core_event_fmt_threshold_comb;
+          i2c_core_event_rx_threshold_comb; i2c_core_event_fmt_overflow_comb;
+          i2c_core_event_rx_overflow_comb; i2c_core_event_nak_comb;
+          i2c_core_event_scl_interference_comb; i2c_core_event_sda_interference_comb;
+          i2c_core_event_stretch_timeout_comb; i2c_core_event_sda_unstable_comb;
+          i2c_core_event_cmd_complete_comb; i2c_core_event_tx_stretch_comb;
+          i2c_core_event_tx_overflow_comb; i2c_core_event_acq_full_comb;
+          i2c_core_event_unexp_stop_comb; i2c_core_event_host_timeout_comb;
+          i2c_core_hw2reg_intr_state_fmt_threshold_de_comb;
+          i2c_core_hw2reg_intr_state_fmt_threshold_d_comb;
+          i2c_core_hw2reg_intr_state_rx_threshold_de_comb;
+          i2c_core_hw2reg_intr_state_rx_threshold_d_comb;
+          i2c_core_hw2reg_intr_state_fmt_overflow_de_comb;
+          i2c_core_hw2reg_intr_state_fmt_overflow_d_comb;
+          i2c_core_hw2reg_intr_state_rx_overflow_de_comb;
+          i2c_core_hw2reg_intr_state_rx_overflow_d_comb;
+          i2c_core_hw2reg_intr_state_nak_de_comb; i2c_core_hw2reg_intr_state_nak_d_comb;
+          i2c_core_hw2reg_intr_state_scl_interference_de_comb;
+          i2c_core_hw2reg_intr_state_scl_interference_d_comb;
+          i2c_core_hw2reg_intr_state_sda_interference_de_comb;
+          i2c_core_hw2reg_intr_state_sda_interference_d_comb;
+          i2c_core_hw2reg_intr_state_stretch_timeout_de_comb;
+          i2c_core_hw2reg_intr_state_stretch_timeout_d_comb;
+          i2c_core_hw2reg_intr_state_sda_unstable_de_comb;
+          i2c_core_hw2reg_intr_state_sda_unstable_d_comb;
+          i2c_core_hw2reg_intr_state_cmd_complete_de_comb;
+          i2c_core_hw2reg_intr_state_cmd_complete_d_comb;
+          i2c_core_hw2reg_intr_state_tx_stretch_de_comb;
+          i2c_core_hw2reg_intr_state_tx_stretch_d_comb;
+          i2c_core_hw2reg_intr_state_tx_overflow_de_comb;
+          i2c_core_hw2reg_intr_state_tx_overflow_d_comb;
+          i2c_core_hw2reg_intr_state_acq_full_de_comb;
+          i2c_core_hw2reg_intr_state_acq_full_d_comb;
+          i2c_core_hw2reg_intr_state_unexp_stop_de_comb;
+          i2c_core_hw2reg_intr_state_unexp_stop_d_comb;
+          i2c_core_hw2reg_intr_state_host_timeout_de_comb;
+          i2c_core_hw2reg_intr_state_host_timeout_d_comb; i2c_core_next_stretch_idle_cnt;
+          next_pend_restart_comb; next_trans_started_comb; next_bit_index_comb;
+          i2c_core_status_fmtfull_d_comb; i2c_core_status_rxfull_d_comb;
+          i2c_core_status_fmtempty_d_comb; i2c_core_status_hostidle_d_comb;
+          i2c_core_status_targetidle_d_comb; i2c_core_status_rxempty_d_comb;
+          i2c_core_rdata_rdata_d_comb; i2c_core_fifo_status_fmtlvl_d_comb;
+          i2c_core_fifo_status_rxlvl_d_comb; i2c_core_val_scl_rx_d_comb;
+          i2c_core_val_sda_rx_d_comb; i2c_core_status_txfull_d_comb;
+          i2c_core_status_acqfull_d_comb; i2c_core_status_txempty_d_comb;
+          i2c_core_status_acqempty_d_comb; i2c_core_fifo_status_txlvl_d_comb;
+          i2c_core_fifo_status_acqlvl_d_comb; i2c_core_acqdata_abyte_d_comb;
+          i2c_core_acqdata_signal_d_comb;
           i2c_reg_top_comb_2]))
        i2c_circuit_init
 Proof
@@ -152,11 +157,12 @@ local
     "intr_unexp_stop_o",
     "intr_host_timeout_o"
   ];
-  val comms = i2c_reg_comms @ [];
   val comms = i2c_reg_comms @ ["fsm_state", "counter", "stretch_idle_cnt", "under_rst", "fmt_fifo_rptr", "fmt_fifo_wptr", "fmt_fifo_regfile",
-                             "rx_fifo_regfile", "rx_fifo_rptr", "rx_fifo_wptr", "bit_index", "pend_restart", "byte_index", "trans_started",
+                             "rx_fifo_regfile", "rx_fifo_rptr", "rx_fifo_wptr", "tx_fifo_regfile", "tx_fifo_rptr", "tx_fifo_wptr",
+                             "acq_fifo_regfile", "acq_fifo_rptr", "acq_fifo_wptr", "bit_index", "pend_restart", "byte_index", "trans_started",
                              "read_byte", "sda_rx_val", "scl_rx_val", "scl_buf", "sda_buf", "scl_sync", "sda_sync", "input_byte", "bit_idx",
-                             "rw_bit", "host_ack"]
+                             "rw_bit", "host_ack", "scl_i_q", "sda_i_q", "fmt_threshold_q", "rx_threshold_q", "sda_rise_cnt", "scl_q",
+                             "sda_q", "test_tx_stretch", "test_acq_full"]
 
 in
   val tstate = init_translator i2c_circuit_alt_def [] comms;
